\documentclass[a4paper, 12pt]{scrartcl}
\usepackage[utf8]{inputenc}
\usepackage[T1]{fontenc}
\usepackage{lmodern}
\usepackage{amsmath}
\newcommand{\deriv}[1]{\ensuremath{\frac{\mathrm{d}}}{\mathrm{d}{#1}}}

\begin{document}

\[
 y^\prime(x) = \deriv{x}\left(f(x)(1 + kg(x))\right) = (1 + kg(x))\deriv{x}f(x) + f(x) k\deriv{x}g(x)
\]


\[
 y^\prime(x) - (1 + kg(x))\deriv{x}f(x) = f(x) k\deriv{x}g(x)
\]

\[
 \frac{y^\prime(x) - (1 + kg(x))\deriv{x}f(x)}{f(x) k} =\deriv{x}g(x)
\]

To be computed in $x=x_0$ and $x=x_1$.

\end{document}
