\documentclass[a4paper, 12pt]{scrartcl}
\usepackage[utf8]{inputenc}
\usepackage[T1]{fontenc}
\usepackage{lmodern}
\usepackage{amsmath}

\title{A growth model}
\author{Torbj√∂rn Rathsman}

\begin{document}
\maketitle
\section{Quantities}
\subsection{State variables}
\begin{tabular}{ll}
$b$ & Current biomass \\
$r$ & Current amount of resources
\end{tabular}
\subsection{Model parameters}
\begin{tabular}{ll}
  $g_b$ & Biomass growth rate \\
 $d_b$ & Biomass death rate \\
 $c_{rb}$ & Resource consumption rate \\
 $e_r$ & Resource evaporation rate \\
 $s_r$ & Resource spawn rate \\
\end{tabular}

\section{Model}
\begin{equation}
M=
\left\{
 \begin{aligned}
  \dot{b} &= g_b rb - d_b b =  b g_b\left(r - \frac{d_b}{g_b}\right) = b g_b\left(r - r_c\right) \\
  \dot{r} &= -c_{rb} r b - e_r r + r_g = -rc_{rb}\left(b + \frac{e_r}{c_{rb}}\right) +s_r = -rc_{rb}\left(b + b_0\right) +s_r
 \end{aligned}
 \right.
\end{equation}

\section{Fixed points}
\paragraph{If $b = 0$ (Uninteresting)}
\[
 0 = -b_0c_{rb}r + s_r \Leftrightarrow r = \frac{s_r}{b_0 c_{rb}}
\]

\paragraph{If $r = r_c$}
\[
 0 = -r_c c_{rb}\left(b + b_0\right) + s_r \Leftrightarrow b + b_0 = \frac{s_r}{r_c c_{rb}} \Leftrightarrow b =
 \frac{s_r}{r_c c_{rb}} - b_0 =  \frac{s_r - r_c c_{rb}b_0}{r_c c_{rb}}
\]

\section{Stability}
\begin{equation}
J(M) =
 \begin{bmatrix}
 g_b\left(r - r_c\right) & bg_b\\
 -rc_{rb} & -c_{rb}\left(b + b_0\right)
 \end{bmatrix}
\end{equation}

\[
\begin{aligned}
0 &= \left(g_b\left(r - r_c\right) - \lambda\right)\left(-c_{rb}\left(b + b_0\right) - \lambda\right) +bg_b r c_{rb} =_{\left\{r = r_c\right\}}\\
  &= \lambda\left(c_{rb}\left(b + b_0\right) + \lambda\right) +bg_b r c_{rb} = \lambda^2 + \lambda c_{rb}\left(b + b_0\right) + bg_b r_c c_{rb} =_{\left\{b + b_0 = \frac{s_r}{r_c c_{rb}}\right\}}\\
  &= \lambda^2 + \lambda \frac{s_r}{r_c} + bg_b r c_{rb} \Leftrightarrow \\
\lambda^2 + \lambda \frac{s_r}{r_c} &= -bg_b r_c c_{rb} \\
&\Leftrightarrow \left(\lambda + \frac{s_r}{2r_c}\right)^2 - \frac{s_r^2}{4r_c^2} = -bg_b r_c c_{rb}\\
&\Leftrightarrow \left(\lambda + \frac{s_r}{2r_c}\right)^2  = \frac{s_r^2}{4r_c^2} -bg_b r_c c_{rb}\\
&\Leftrightarrow_{\left\{b = \frac{s_r - r_c c_{rb}b_0}{r_c c_{rb}}\right\}} \left(\lambda + \frac{s_r}{2r_c}\right)^2  = \frac{s_r^2}{4r_c^2} -\frac{s_r - r_c c_{rb}b_0}{r_c c_{rb}}g_b r_c c_{rb} = \frac{s_r^2}{4r_c^2} -\left(s_r - r_c c_{rb}b_0\right)g_b \\
\end{aligned}
\]
\[
\begin{aligned}
 \lambda_1 &= -\frac{s_r}{2r_c}-\sqrt{\frac{s_r^2}{4r_c^2} - \left(s_r - r_c c_{rb}b_0\right)g_b} \\
 \lambda_2 &= -\frac{s_r}{2r_c}+\sqrt{\frac{s_r^2}{4r_c^2} - \left(s_r - r_c c_{rb}b_0\right)g_b} \\
\end{aligned}
\]

With sufficiently large $g_b$, this is a stable spiral.


\end{document}
